@prefix cms: <http://mu.semte.ch/vocabulary/cms/>.
@prefix cycling: <http://mu.semte.ch/vocabularies/ext/cycing/>.
@prefix lmb: <http://lblod.data.gift/vocabularies/lmb/>.
@prefix nao: <http://www.semanticdesktop.org/ontologies/2007/08/15/nao#>.
@prefix eli: <http://data.europa.eu/eli/ontology#>.
@prefix extlmb: <http://mu.semte.ch/vocabularies/ext/lmb/>.
@prefix mu: <http://mu.semte.ch/vocabularies/core/>.
@prefix sh: <http://www.w3.org/ns/shacl#>.
@prefix form: <http://lblod.data.gift/vocabularies/forms/>.
@prefix euvoc: <http://publications.europa.eu/ontology/euvoc#>.
@prefix ch: <http://data.lblod.info/vocabularies/contacthub/>.
@prefix rdfs: <http://www.w3.org/2000/01/rdf-schema#>.
@prefix adres: <https://data.vlaanderen.be/ns/adres#>.
@prefix locn: <http://www.w3.org/ns/locn#>.
@prefix lblodlg: <http://data.lblod.info/vocabularies/leidinggevenden/>.
@prefix dbpedia: <http://dbpedia.org/ontology/>.
@prefix schema: <http://schema.org/>.
@prefix nie: <http://www.semanticdesktop.org/ontologies/2007/01/19/nie#>.
@prefix nfo: <http://www.semanticdesktop.org/ontologies/2007/03/22/nfo#>.
@prefix foaf: <http://xmlns.com/foaf/0.1/>.
@prefix skos: <http://www.w3.org/2004/02/skos/core#>.
@prefix regorg: <https://www.w3.org/ns/regorg#>.
@prefix prov: <http://www.w3.org/ns/prov#>.
@prefix org: <http://www.w3.org/ns/org#>.
@prefix person: <http://www.w3.org/ns/person#>.
@prefix adms: <http://www.w3.org/ns/adms#>.
@prefix dct: <http://purl.org/dc/terms/>.
@prefix generiek: <http://data.vlaanderen.be/ns/generiek#>.
@prefix persoon: <http://data.vlaanderen.be/ns/persoon#>.
@prefix mandaat: <http://data.vlaanderen.be/ns/mandaat#>.
@prefix besluit: <http://data.vlaanderen.be/ns/besluit#>.
@prefix ext: <http://mu.semte.ch/vocabularies/ext/>.
@prefix rm: <http://mu.semte.ch/vocabularies/logical-delete/>.
@prefix typedLiterals: <http://mu.semte.ch/vocabularies/typed-literals/>.
@prefix xsd: <http://www.w3.org/2001/XMLSchema#>.
@prefix app: <http://mu.semte.ch/app/>.
@prefix owl: <http://www.w3.org/2002/07/owl#>.
@prefix rdf: <http://www.w3.org/1999/02/22-rdf-syntax-ns#>.
@prefix dc: <http://purl.org/dc/elements/1.1/>.

<http://mu.semte.ch/ontology> rdf:type owl:Ontology.
<http://mu.semte.ch/ontology> dc:title "Generated resource ontology". 
<http://mu.semte.ch/ontology> dc:description "Generated resource ontology". 

cycling:RouteSectie rdf:type owl:Class;
  rdfs:label "route-section".
prov:Location rdf:type owl:Class;
  rdfs:label "werkingsgebied".
foaf:Person rdf:type owl:Class;
  rdfs:label "gebruiker".
skos:Concept rdf:type owl:Class;
  rdfs:label "concept".
cycling:GoedkeuringDoorGemeente rdf:type owl:Class;
  rdfs:label "approval-by-commune".
locn:Address rdf:type owl:Class;
  rdfs:label "adres".
besluit:Agendapunt rdf:type owl:Class;
  rdfs:label "agendapunt".
besluit:Besluit rdf:type owl:Class;
  rdfs:label "besluit".
besluit:BehandelingVanAgendapunt rdf:type owl:Class;
  rdfs:label "behandeling-van-agendapunt".
foaf:OnlineAccount rdf:type owl:Class;
  rdfs:label "account".
cycling:RequestStateClassification rdf:type owl:Class;
   rdfs:subClassOf skos:Concept;
  rdfs:label "request-state-classification".
sign:PublishedResource rdf:type owl:Class;
  rdfs:label "published-resource".
cycling:Aanvraag rdf:type owl:Class;
  rdfs:label "cycling-request".
besluit:Bestuurseenheid rdf:type owl:Class;
  rdfs:label "bestuurseenheid".
skos:ConceptScheme rdf:type owl:Class;
  rdfs:label "concept-scheme".
ext:BestuurseenheidClassificatieCode rdf:type owl:Class;
  rdfs:label "bestuurseenheid-classificatie-code".

ext:local_id_1 rdf:type owl:DatatypeProperty;
  rdfs:comment "Resources type is datetime.  Original predicate is dct:createdAt.";
  rdfs:label "created";
  rdfs:range rdfs:Literal;
  rdfs:domain cycling:Aanvraag.
ext:local_id_2 rdf:type owl:DatatypeProperty;
  rdfs:comment "Resources type is datetime.  Original predicate is dct:createdAt.";
  rdfs:label "created";
  rdfs:range rdfs:Literal;
  rdfs:domain cycling:GoedkeuringDoorGemeente.
ext:local_id_3 rdf:type owl:DatatypeProperty;
  rdfs:comment "Resources type is datetime.  Original predicate is dct:createdAt.";
  rdfs:label "created";
  rdfs:range rdfs:Literal;
  rdfs:domain cycling:RouteSectie.
cycling:startPassage rdf:type owl:DatatypeProperty;
  rdfs:comment "Resources type is datetime.  Original predicate is cycling:startPassage.";
  rdfs:label "time-of-passing-start";
  rdfs:range rdfs:Literal;
  rdfs:domain cycling:RouteSectie.
cycling:endPassage rdf:type owl:DatatypeProperty;
  rdfs:comment "Resources type is datetime.  Original predicate is cycling:endPassage.";
  rdfs:label "time-of-passing-end";
  rdfs:range rdfs:Literal;
  rdfs:domain cycling:RouteSectie.
cycling:afstand rdf:type owl:DatatypeProperty;
  rdfs:comment "Resources type is number.  Original predicate is cycling:afstand.";
  rdfs:label "distance";
  rdfs:range rdfs:Literal;
  rdfs:domain cycling:RouteSectie.
rdfs:label rdf:type owl:DatatypeProperty;
  rdfs:comment "Resources type is string.  Original predicate is rdfs:label.";
  rdfs:label "naam";
  rdfs:range rdfs:Literal;
  rdfs:domain prov:Location.
ext:werkingsgebiedNiveau rdf:type owl:DatatypeProperty;
  rdfs:comment "Resources type is string.  Original predicate is ext:werkingsgebiedNiveau.";
  rdfs:label "niveau";
  rdfs:range rdfs:Literal;
  rdfs:domain prov:Location.
foaf:firstName rdf:type owl:DatatypeProperty;
  rdfs:comment "Resources type is string.  Original predicate is foaf:firstName.";
  rdfs:label "voornaam";
  rdfs:range rdfs:Literal;
  rdfs:domain foaf:Person.
foaf:familyName rdf:type owl:DatatypeProperty;
  rdfs:comment "Resources type is string.  Original predicate is foaf:familyName.";
  rdfs:label "achternaam";
  rdfs:range rdfs:Literal;
  rdfs:domain foaf:Person.
ext:local_id_4 rdf:type owl:DatatypeProperty;
  rdfs:comment "Resources type is via.  Original predicate is dct:identifier.";
  rdfs:label "vo-id";
  rdfs:range rdfs:Literal;
  rdfs:domain foaf:OnlineAccount.
ext:local_id_5 rdf:type owl:DatatypeProperty;
  rdfs:comment "Resources type is string.  Original predicate is dct:identifier.";
  rdfs:label "rijksregister-nummer";
  rdfs:range rdfs:Literal;
  rdfs:domain foaf:Person.
ext:local_id_6 rdf:type owl:DatatypeProperty;
  rdfs:comment "Resources type is string.  Original predicate is skos:prefLabel.";
  rdfs:label "label";
  rdfs:range rdfs:Literal;
  rdfs:domain ext:BestuurseenheidClassificatieCode.
ext:local_id_7 rdf:type owl:DatatypeProperty;
  rdfs:comment "Resources type is string.  Original predicate is skos:prefLabel.";
  rdfs:label "label";
  rdfs:range rdfs:Literal;
  rdfs:domain skos:ConceptScheme.
ext:local_id_8 rdf:type owl:DatatypeProperty;
  rdfs:comment "Resources type is string.  Original predicate is skos:prefLabel.";
  rdfs:label "naam";
  rdfs:range rdfs:Literal;
  rdfs:domain besluit:Bestuurseenheid.
ext:local_id_9 rdf:type owl:DatatypeProperty;
  rdfs:comment "Resources type is string.  Original predicate is skos:prefLabel.";
  rdfs:label "label";
  rdfs:range rdfs:Literal;
  rdfs:domain skos:Concept.
adres:Adresvoorstelling.busnummer rdf:type owl:DatatypeProperty;
  rdfs:comment "Resources type is string.  Original predicate is adres:Adresvoorstelling.busnummer.";
  rdfs:label "busnummer";
  rdfs:range rdfs:Literal;
  rdfs:domain locn:Address.
adres:AdresVoorstelling.huisnummer rdf:type owl:DatatypeProperty;
  rdfs:comment "Resources type is string.  Original predicate is adres:AdresVoorstelling.huisnummer.";
  rdfs:label "huisnummer";
  rdfs:range rdfs:Literal;
  rdfs:domain locn:Address.
locn:thoroughfare rdf:type owl:DatatypeProperty;
  rdfs:comment "Resources type is string.  Original predicate is locn:thoroughfare.";
  rdfs:label "straatnaam";
  rdfs:range rdfs:Literal;
  rdfs:domain locn:Address.
locn:postCode rdf:type owl:DatatypeProperty;
  rdfs:comment "Resources type is string.  Original predicate is locn:postCode.";
  rdfs:label "postcode";
  rdfs:range rdfs:Literal;
  rdfs:domain locn:Address.
adres:gemeentenaam rdf:type owl:DatatypeProperty;
  rdfs:comment "Resources type is string.  Original predicate is adres:gemeentenaam.";
  rdfs:label "gemeentenaam";
  rdfs:range rdfs:Literal;
  rdfs:domain locn:Address.
adres:land rdf:type owl:DatatypeProperty;
  rdfs:comment "Resources type is language-string-set.  Original predicate is adres:land.";
  rdfs:label "land";
  rdfs:range rdfs:Literal;
  rdfs:domain locn:Address.
locn:locatorDesignator rdf:type owl:DatatypeProperty;
  rdfs:comment "Resources type is string.  Original predicate is locn:locatorDesignator.";
  rdfs:label "locatieaanduiding";
  rdfs:range rdfs:Literal;
  rdfs:domain locn:Address.
locn:locatorName rdf:type owl:DatatypeProperty;
  rdfs:comment "Resources type is language-string-set.  Original predicate is locn:locatorName.";
  rdfs:label "locatienaam";
  rdfs:range rdfs:Literal;
  rdfs:domain locn:Address.
locn:poBox rdf:type owl:DatatypeProperty;
  rdfs:comment "Resources type is string.  Original predicate is locn:poBox.";
  rdfs:label "postbus";
  rdfs:range rdfs:Literal;
  rdfs:domain locn:Address.
locn:postName rdf:type owl:DatatypeProperty;
  rdfs:comment "Resources type is string.  Original predicate is locn:postName.";
  rdfs:label "postnaam";
  rdfs:range rdfs:Literal;
  rdfs:domain locn:Address.
locn:fullAddress rdf:type owl:DatatypeProperty;
  rdfs:comment "Resources type is string.  Original predicate is locn:fullAddress.";
  rdfs:label "volledig-adres";
  rdfs:range rdfs:Literal;
  rdfs:domain locn:Address.
lblodlg:adresRegisterId rdf:type owl:DatatypeProperty;
  rdfs:comment "Resources type is number.  Original predicate is lblodlg:adresRegisterId.";
  rdfs:label "adres-register-id";
  rdfs:range rdfs:Literal;
  rdfs:domain locn:Address.
adres:verwijstNaar rdf:type owl:DatatypeProperty;
  rdfs:comment "Resources type is url.  Original predicate is adres:verwijstNaar.";
  rdfs:label "adres-register-uri";
  rdfs:range rdfs:Literal;
  rdfs:domain locn:Address.
dct:description rdf:type owl:DatatypeProperty;
  rdfs:comment "Resources type is string.  Original predicate is dct:description.";
  rdfs:label "beschrijving";
  rdfs:range rdfs:Literal;
  rdfs:domain besluit:Agendapunt.
dct:title rdf:type owl:DatatypeProperty;
  rdfs:comment "Resources type is string.  Original predicate is dct:title.";
  rdfs:label "titel";
  rdfs:range rdfs:Literal;
  rdfs:domain besluit:Agendapunt.
besluit:Agendapunt.type rdf:type owl:DatatypeProperty;
  rdfs:comment "Resources type is uri-set.  Original predicate is besluit:Agendapunt.type.";
  rdfs:label "type";
  rdfs:range rdfs:Literal;
  rdfs:domain besluit:Agendapunt.
eli:description rdf:type owl:DatatypeProperty;
  rdfs:comment "Resources type is string.  Original predicate is eli:description.";
  rdfs:label "beschrijving";
  rdfs:range rdfs:Literal;
  rdfs:domain besluit:Besluit.
eli:title_short rdf:type owl:DatatypeProperty;
  rdfs:comment "Resources type is string.  Original predicate is eli:title_short.";
  rdfs:label "citeeropschrift";
  rdfs:range rdfs:Literal;
  rdfs:domain besluit:Besluit.
besluit:motivering rdf:type owl:DatatypeProperty;
  rdfs:comment "Resources type is string.  Original predicate is besluit:motivering.";
  rdfs:label "motivering";
  rdfs:range rdfs:Literal;
  rdfs:domain besluit:Besluit.
eli:date_publication rdf:type owl:DatatypeProperty;
  rdfs:comment "Resources type is date.  Original predicate is eli:date_publication.";
  rdfs:label "publicatiedatum";
  rdfs:range rdfs:Literal;
  rdfs:domain besluit:Besluit.
prov:value rdf:type owl:DatatypeProperty;
  rdfs:comment "Resources type is string.  Original predicate is prov:value.";
  rdfs:label "inhoud";
  rdfs:range rdfs:Literal;
  rdfs:domain besluit:Besluit.
eli:language rdf:type owl:DatatypeProperty;
  rdfs:comment "Resources type is url.  Original predicate is eli:language.";
  rdfs:label "taal";
  rdfs:range rdfs:Literal;
  rdfs:domain besluit:Besluit.
eli:title rdf:type owl:DatatypeProperty;
  rdfs:comment "Resources type is string.  Original predicate is eli:title.";
  rdfs:label "titel";
  rdfs:range rdfs:Literal;
  rdfs:domain besluit:Besluit.
nao:score rdf:type owl:DatatypeProperty;
  rdfs:comment "Resources type is float.  Original predicate is nao:score.";
  rdfs:label "score";
  rdfs:range rdfs:Literal;
  rdfs:domain besluit:Besluit.
foaf:accountServiceHomepage rdf:type owl:DatatypeProperty;
  rdfs:comment "Resources type is via.  Original predicate is foaf:accountServiceHomepage.";
  rdfs:label "provider";
  rdfs:range rdfs:Literal;
  rdfs:domain foaf:OnlineAccount.
sign:text rdf:type owl:DatatypeProperty;
  rdfs:comment "Resources type is string.  Original predicate is sign:text.";
  rdfs:label "content";
  rdfs:range rdfs:Literal;
  rdfs:domain sign:PublishedResource.
skos:altLabel rdf:type owl:DatatypeProperty;
  rdfs:comment "Resources type is string-set.  Original predicate is skos:altLabel.";
  rdfs:label "alternatieve-naam";
  rdfs:range rdfs:Literal;
  rdfs:domain besluit:Bestuurseenheid.
ext:wilMailOntvangen rdf:type owl:DatatypeProperty;
  rdfs:comment "Resources type is boolean.  Original predicate is ext:wilMailOntvangen.";
  rdfs:label "wil-mail-ontvangen";
  rdfs:range rdfs:Literal;
  rdfs:domain besluit:Bestuurseenheid.
ext:mailAdresVoorNotificaties rdf:type owl:DatatypeProperty;
  rdfs:comment "Resources type is string.  Original predicate is ext:mailAdresVoorNotificaties.";
  rdfs:label "mail-adres";
  rdfs:range rdfs:Literal;
  rdfs:domain besluit:Bestuurseenheid.
skos:scopeNote rdf:type owl:DatatypeProperty;
  rdfs:comment "Resources type is string.  Original predicate is skos:scopeNote.";
  rdfs:label "scope-note";
  rdfs:range rdfs:Literal;
  rdfs:domain ext:BestuurseenheidClassificatieCode.


cycling:gebruiktWerkingsgebied rdf:type owl:ObjectProperty;
  rdfs:comment "";
  rdfs:label "areas";
  rdfs:domain cycling:RouteSectie;
  rdfs:range locn:Address.
besluit:werkingsgebied rdf:type owl:ObjectProperty;
  rdfs:comment "";
  rdfs:label "werkingsgebied";
  rdfs:domain besluit:Bestuurseenheid;
  rdfs:range prov:Location.
foaf:account rdf:type owl:ObjectProperty;
  rdfs:comment "";
  rdfs:label "account";
  rdfs:domain foaf:Person;
  rdfs:range foaf:OnlineAccount.
skos:inScheme rdf:type owl:ObjectProperty;
  rdfs:comment "";
  rdfs:label "concept-schemes";
  rdfs:domain skos:Concept;
  rdfs:range skos:ConceptScheme.
skos:topConceptOf rdf:type owl:ObjectProperty;
  rdfs:comment "";
  rdfs:label "top-concept-schemes";
  rdfs:domain skos:Concept;
  rdfs:range skos:ConceptScheme.
cycling:bevoegdeBestuurseenheid rdf:type owl:ObjectProperty;
  rdfs:comment "";
  rdfs:label "municipality";
  rdfs:domain cycling:GoedkeuringDoorGemeente;
  rdfs:range besluit:Bestuurseenheid.
cycling:afweging rdf:type owl:ObjectProperty;
  rdfs:comment "";
  rdfs:label "consideration";
  rdfs:domain cycling:GoedkeuringDoorGemeente;
  rdfs:range besluit:Agendapunt.
cycling:innameOpenbaarDomein rdf:type owl:ObjectProperty;
  rdfs:comment "";
  rdfs:label "taking-domain";
  rdfs:domain cycling:GoedkeuringDoorGemeente;
  rdfs:range besluit:Agendapunt.
cycling:approvalByMayor rdf:type owl:ObjectProperty;
  rdfs:comment "";
  rdfs:label "approval-mayor";
  rdfs:domain cycling:GoedkeuringDoorGemeente;
  rdfs:range besluit:Agendapunt.
prov:wasDerivedFrom rdf:type owl:ObjectProperty;
  rdfs:comment "";
  rdfs:label "publications";
  rdfs:domain besluit:Agendapunt;
  rdfs:range sign:PublishedResource.
besluit:aangebrachtNa rdf:type owl:ObjectProperty;
  rdfs:comment "";
  rdfs:label "vorige-agendapunt";
  rdfs:domain besluit:Agendapunt;
  rdfs:range besluit:Agendapunt.
dct:subject rdf:type owl:ObjectProperty;
  rdfs:comment "";
  rdfs:label "onderwerp";
  rdfs:domain besluit:BehandelingVanAgendapunt;
  rdfs:range besluit:Agendapunt.
prov:generated rdf:type owl:ObjectProperty;
  rdfs:comment "";
  rdfs:label "besluiten";
  rdfs:domain besluit:BehandelingVanAgendapunt;
  rdfs:range besluit:Besluit.
besluit:gebeurtNa rdf:type owl:ObjectProperty;
  rdfs:comment "";
  rdfs:label "vorige-behandeling-van-agendapunt";
  rdfs:domain besluit:BehandelingVanAgendapunt;
  rdfs:range besluit:BehandelingVanAgendapunt.
cylcing:state rdf:type owl:ObjectProperty;
  rdfs:comment "";
  rdfs:label "requests";
  rdfs:domain cycling:Aanvraag;
  rdfs:range cycling:RequestStateClassification.
cycling:routeSectie rdf:type owl:ObjectProperty;
  rdfs:comment "";
  rdfs:label "route-sections";
  rdfs:domain cycling:Aanvraag;
  rdfs:range cycling:RouteSectie.
cycling:state rdf:type owl:ObjectProperty;
  rdfs:comment "";
  rdfs:label "state";
  rdfs:domain cycling:Aanvraag;
  rdfs:range cycling:RequestStateClassification.
besluit:classificatie rdf:type owl:ObjectProperty;
  rdfs:comment "";
  rdfs:label "classificatie";
  rdfs:domain besluit:Bestuurseenheid;
  rdfs:range ext:BestuurseenheidClassificatieCode.



